src/Utils/TrieMapInt63.v
@@ -1,0 +1,243 @@
+Require Import ZArith Int63.
+Open Scope int63.
+Require Import coqutil.Map.Interface.
+Require Import Tries.Canonical.
+Import PTree.
+
+Require Utils.ArrayList Utils.TrieMap.
+(*
+(* positives consed when they should be appended*)
+Fixpoint trie_fold' {B A} (f : A -> positive -> B -> A) (acc : A) (m : PTree.tree' B)
+         (*TODO: find a better way*)
+         (num : positive -> positive) : A :=
+  match m with
+  | Node001 r => trie_fold' f acc r (fun a => num (xI a))
+  | Node010 y => f acc (num xH) y
+  | Node011 y r =>
+      let acc := f acc (num xH) y in
+      trie_fold' f acc r (fun a => num (xI a))
+  | Node100 l => trie_fold' f acc l (fun a => num (xO a))
+  | Node101 l r =>      
+      let acc := trie_fold' f acc r (fun a => num (xI a)) in
+      trie_fold' f acc l (fun a => num (xO a))
+  | Node110 l y => 
+      let acc := f acc (num xH) y in
+      trie_fold' f acc l (fun a => num (xO a))
+  | Node111 l y r =>
+      let acc := f acc (num xH) y in
+      let acc := trie_fold' f acc r (fun a => num (xI a)) in
+      trie_fold' f acc l (fun a => num (xO a))
+end.
+
+
+Definition trie_fold {B A} (f : A -> positive -> B -> A) (acc : A) (m : PTree.t B) : A :=
+  match m with
+  | Empty => acc
+  | Nodes m' => trie_fold' f acc m' id
+  end.
+  
+ *)
+
+(** PTree operations reimplemented for i63.
+    Note that we can't differentiate between 0 and 000 by default,
+    so we trim all leading 0s to avoid making each access have depth 64.
+ *)
+
+(* Note: this can be expensive for large numbers, should only be called on small ones.
+   Invariant: this file only calls it on numbers <= digits
+ *)
+Local Definition int_to_nat (i : int) := Z.to_nat (Uint63.to_Z i).
+
+Fixpoint get' {A} (p: int) (m: tree' A) (msb : nat) : option A :=
+  let q := p >> 1 in
+  match msb, m, is_zero (p land 1) with
+  | O, Node001 _, _ => None
+  | O, Node010 x, _ => Some x
+  | O, Node011 x _, _ => Some x
+  | O, Node100 _, _ => None
+  | O, Node101 _ _, _ => None
+  | O, Node110 _ x, _ => Some x
+  | O, Node111 _ x _, _ => Some x
+  | S msb, Node001 _, true => None
+  | S msb, Node010 _, true => None
+  | S msb, Node011 _ _, true => None
+  | S msb, Node100 m', true => get' q m' msb
+  | S msb, Node101 m' _, true => get' q m' msb
+  | S msb, Node110 m' _, true => get' q m' msb
+  | S msb, Node111 m' _ _, true => get' q m' msb
+  | S msb, Node001 m', false => get' q m' msb
+  | S msb, Node010 _, false => None
+  | S msb, Node011 _ m', false => get' q m' msb
+  | S msb, Node100 m', false => None
+  | S msb, Node101 _ m', false => get' q m' msb
+  | S msb, Node110 _ _, false => None
+  | S msb, Node111 _ _ m', false => get' q m' msb
+  end.
+
+(* TODO: we always use int_to_nat (msb p). Should we implement that directly?
+   It would probably be faster.
+ *)
+Definition msb i := digits - (head0 i).
+
+Definition get {A} (m : tree A) (p: int) : option A :=
+  match m with
+  | Empty => None
+  | Nodes m' => get' p m' (int_to_nat (msb p))
+  end.
+
+Fixpoint set0 {A} (p: int) (x: A) (msb : nat) : tree' A :=
+  let q := p >> 1 in
+  match msb, is_zero (p land 1) with
+  | O, _ => Node010 x
+  | S msb, true => Node100 (set0 q x msb)
+  | S msb, false => Node001 (set0 q x msb)
+  end.
+
+Fixpoint set' {A} (p: int) (x: A) (m: tree' A) (msb : nat) : tree' A :=
+  let q := p >> 1 in
+match msb, m, is_zero (p land 1) with
+| O, Node001 r, _ => Node011 x r
+| O, Node010 _, _ => Node010 x
+| O, Node011 _ r, _ => Node011 x r
+| O, Node100 l, _ => Node110 l x
+| O, Node101 l r, _ => Node111 l x r
+| O, Node110 l _, _ => Node110 l x
+| O, Node111 l _ r, _ => Node111 l x r
+| S msb, Node001 r, true => Node101 (set0 q x msb) r
+| S msb, Node010 y, true => Node110 (set0 q x msb) y
+| S msb, Node011 y r, true => Node111 (set0 q x msb) y r
+| S msb, Node100 l, true => Node100 (set' q x l msb)
+| S msb, Node101 l r, true => Node101 (set' q x l msb) r
+| S msb, Node110 l y, true => Node110 (set' q x l msb) y
+| S msb, Node111 l y r, true => Node111 (set' q x l msb) y r
+| S msb, Node001 r, false => Node001 (set' q x r msb)
+| S msb, Node010 y, false => Node011 y (set0 q x msb)
+| S msb, Node011 y r, false => Node011 y (set' q x r msb)
+| S msb, Node100 l, false => Node101 l (set0 q x msb)
+| S msb, Node101 l r, false => Node101 l (set' q x r msb)
+| S msb, Node110 l y, false => Node111 l y (set0 q x msb)
+| S msb, Node111 l y r, false => Node111 l y (set' q x r msb)
+end.
+
+Definition set {A} (m: tree A) (p: int) (x: A) : tree A :=
+match m with
+| Empty => Nodes (set0 p x (int_to_nat (msb p)))
+| Nodes m' => Nodes (set' p x m' (int_to_nat (msb p)))
+end.
+
+
+Fixpoint rem' {A} (p: int) (m: tree' A) (msb : nat) : tree A :=
+  let q := p >> 1 in
+  match msb, m, is_zero (p land 1) with
+  | O, Node001 r,_ => Nodes m
+  | O, Node010 _,_ => Empty
+  | O, Node011 _ r,_ => Nodes (Node001 r)
+  | O, Node100 l,_ => Nodes m
+  | O, Node101 l r,_ => Nodes m
+  | O, Node110 l _,_ => Nodes (Node100 l)
+  | O, Node111 l _ r,_ => Nodes (Node101 l r)
+  | S msb, Node001 r, true => Nodes m
+  | S msb, Node010 y, true => Nodes m
+  | S msb, Node011 y r, true => Nodes m
+  | S msb, Node100 l, true => Node (rem' q l msb) None Empty
+  | S msb, Node101 l r, true => Node (rem' q l msb) None (Nodes r)
+  | S msb, Node110 l y, true => Node (rem' q l msb) (Some y) Empty
+  | S msb, Node111 l y r, true => Node (rem' q l msb) (Some y) (Nodes r)
+  | S msb, Node001 r, false => Node Empty None (rem' q r msb)
+  | S msb, Node010 y, false => Nodes m
+  | S msb, Node011 y r, false => Node Empty (Some y) (rem' q r msb)
+  | S msb, Node100 l, false => Nodes m
+  | S msb, Node101 l r, false => Node (Nodes l) None (rem' q r msb)
+  | S msb, Node110 l y, false => Nodes m
+  | S msb, Node111 l y r, false => Node (Nodes l) (Some y) (rem' q r msb)
+  end.
+
+(** This use of [Node] causes some run-time overhead, which we eliminate
+    by asking Coq to unfold the definition of [Node] in [rem'],
+    then simplify the definition.  This is a form of partial evaluation. *)
+
+Definition remove' := Eval cbv [rem' Node] in @rem'.
+
+Definition remove {A} (m: tree A)  (p: int) : tree A :=
+match m with
+| Empty => Empty
+| Nodes m' => remove' _ p m' (int_to_nat (msb p))
+end.
+
+(*
+Fixpoint msb' (fuel : nat) (i : int) : nat * int :=
+  match fuel with
+  (* Should never happen? *)
+  | 0 => (O, 0)
+  | S fuel =>
+      let i' := i >> 1 in
+      if is_zero i'
+      then (O,0)
+      else
+        let (n,i) := msb' fuel i' in
+        (S n, i + 1)
+  end.
+
+Definition msb := msb' size.
+
+(* Note: this should not be used outside this module.
+   It does not represent an principled transformation.
+ (* Note: assumes the input is nonnegative, in which case the function is bijective *)
+ *)
+Local Definition to_pos (i:int) : positive :=
+  (*adding 1 to make sure that 0 gets mapped to a positive. *)
+  match to_Z (i + 1) with
+  | Zpos p => p
+  (*should never happen*)
+  | _ => xH
+  end.
+(*
+  TODO: this is a very poor implementation of fold, improve
+ *)*)
+
+Section __.
+
+  
+  Context (value : Type).
+  
+
+  Section Fold.
+    Context {R : Type} (f : R -> int -> value -> R).
+
+
+    Fixpoint fold' (acc : R) (m : tree' value) (i : int) : R :=
+      (*0 bit ~> left
+        1 bit ~> right
+       *)
+      let i'_l := i << 1 in
+      let i'_r := i'_l lor 1 in
+      match m with
+      | Node001 r => fold' acc r i'_r
+      | Node010 v => f acc i v
+      | Node011 v r => fold' (f acc i v) r i'_r
+      | Node100 l => fold' acc l i'_l
+      | Node101 l r => fold' (fold' acc r i'_r) l i'_l
+      | Node110 l v => fold' (f acc i v) l i'_l
+      | Node111 l v r => fold' (fold' (f acc i v) r i'_r) l i'_l
+      end.
+    
+    Definition fold (acc : R) (m : tree value) : R :=
+      match m with
+      | Empty => acc
+      | Nodes m' => fold' acc m' 0
+      end.
+
+  End Fold.
+
+  Instance map : map.map int value :=
+    {|
+      map.rep := PTree.t value;
+      map.empty := PTree.empty value;
+      map.get := get;
+      map.put := set;
+      map.remove := remove;
+      map.fold := @fold;
+    |}.
+
+  (* TODO: prove map.ok *)
+End __.
